updated obtaining the partial solutions

Licenta.dfy
@@ -5,37 +5,9 @@ predicate hasPositiveValues(input: seq<int>)
     forall i :: 0 <= i < |input| ==> input[i] > 0
 }
 
-function max(p1: int, p2: int): int
+predicate hasOnlyPermittedValues(solution: seq<int>)
 {
-    if p1 > p2 then p1 else p2
-}
-
-function gain(problem: Problem, solution: seq<int>): int
-  requires isValidProblem(problem)
-  requires isValidPartialSolution(problem, solution)
-{
-  if |solution| == 0 then 0 else computeGain(problem.gains, solution, |solution| - 1)
-}
-
-function computeGain(gains: seq<int>, solution: seq<int>, i: int) : int
-  requires 0 <= i < |solution|
-  requires 0 <= i < |gains|
-{
-   if i == 0 then 0 else solution[i] * gains[i] + computeGain(gains, solution, i - 1)
-}
-
-function weight(problem: Problem, solution: seq<int>): int
-  requires isValidProblem(problem)
-  requires isValidPartialSolution(problem, solution)
-{
-  if |solution| == 0 then 0 else computeWeight(problem.weights, solution, |solution| - 1)
-}
-
-function computeWeight(weights: seq<int>, solution: seq<int>, i: int) : int
-  requires 0 <= i < |solution|
-  requires 0 <= i < |weights|
-{
-   if i == 0 then 0 else solution[i] * weights[i] + computeWeight(weights, solution, i - 1)
+  forall k :: 0 <= k < |solution| ==> solution[k] == 0 || solution[k] == 1
 }
 
 predicate isValidProblem(problem: Problem)
@@ -45,20 +17,73 @@ predicate isValidProblem(problem: Problem)
     hasPositiveValues(problem.gains) && hasPositiveValues(problem.weights) 
 }
 
-predicate isValidSolution(problem: Problem, solution: seq<int>)
+function max(p1: int, p2: int): int
 {
-  isValidPartialSolution(problem, solution) &&
+    if p1 > p2 then p1 else p2
+}
+
+function gain(problem: Problem, solution: seq<int>): int
+  requires isValidProblem(problem)
+  requires hasOnlyPermittedValues(solution)
+  requires isValidPartialSolution(problem, solution)
+  requires 0 <= |solution| <= problem.numberOfObjects
+  ensures gain(problem, solution) == if |solution| == 0 then 0 else computeGain(problem.gains, solution, |solution| - 1)
+  // ensures if (forall j :: 0 <= j < |solution| ==> solution[j] == 0) then gain(problem, solution) == 0 else true
+{
+  if |solution| == 0 then 0 else computeGain(problem.gains, solution, |solution| - 1)
+}
+
+function computeGain(gains: seq<int>, solution: seq<int>, i: int) : int
+  requires 0 <= i < |solution|
+  requires 0 <= i < |gains|
+  requires hasOnlyPermittedValues(solution)
+  requires 0 <= |solution| <= |gains|
+  ensures computeGain(gains, solution, i) == if i == 0 then 0 else solution[i] * gains[i] + computeGain(gains, solution, i - 1)
+  // ensures if (forall j :: 0 <= j < |solution| ==> solution[j] == 0) then computeGain(gains, solution, i) == 0 else true
+{
+   if i == 0 then 0 else solution[i] * gains[i] + computeGain(gains, solution, i - 1)
+}
+
+function weight(problem: Problem, solution: seq<int>): int
+  requires isValidProblem(problem)
+  requires hasOnlyPermittedValues(solution)
+  requires 0 <= |solution| <= problem.numberOfObjects
+  ensures weight(problem, solution) == if |solution| == 0 then 0 else computeWeight(problem.weights, solution, |solution| - 1)
+  // ensures if (forall j :: 0 <= j < |solution| ==> solution[j] == 0) then weight(problem, solution) == 0 else true
+{
+  if |solution| == 0 then 0 else computeWeight(problem.weights, solution, |solution| - 1)
+}
+
+function computeWeight(weights: seq<int>, solution: seq<int>, i: int) : int
+  requires 0 <= i < |solution|
+  requires 0 <= i < |weights|
+  requires hasOnlyPermittedValues(solution)
+  requires 0 <= |solution| <= |weights|
+  ensures computeWeight(weights, solution, i) == if i == 0 then 0 else solution[i] * weights[i] + computeWeight(weights, solution, i - 1)
+  // ensures if (forall j :: 0 <= j < |solution| ==> solution[j] == 0) then computeWeight(weights, solution, i) == 0 else true
+{
+   if i == 0 then 0 else solution[i] * weights[i] + computeWeight(weights, solution, i - 1)
+}
+
+predicate isValidSolution(problem: Problem, solution: seq<int>)
+requires isValidProblem(problem)
+requires isValidPartialSolution(problem, solution)
+{
+  isPartialSolution(problem, solution) &&
   |solution| == problem.numberOfObjects
 }
 
 predicate isSolution(p: Problem, solution: seq<int>)
   requires isValidProblem(p)
+  requires isValidPartialSolution(p, solution)
 {
   isValidSolution(p, solution) &&
   weight(p, solution) <= p.knapsackCapacity
 }
 
 predicate isValidPartialSolution(problem: Problem, solution: seq<int>)
+  requires isValidProblem(problem)
+//conditie ca suma obiectelor mai mica decat cap rucsacului
 {
   0 <= |solution| <= problem.numberOfObjects && hasOnlyPermittedValues(solution)
 }
@@ -70,28 +95,24 @@ predicate isPartialSolution(problem: Problem, solution: seq<int>)
   weight(problem, solution) <= problem.knapsackCapacity
 }
 
-ghost predicate isPartialSolutionOfProfit(p: Problem, profit: int, dim: int, partWeight: int)
+ghost predicate existsPartialSolutionOfProfit(p: Problem, profit: int, dim: int, partWeight: int)
   requires isValidProblem(p)
   requires 0 <= dim <= p.numberOfObjects
   requires 0 <= partWeight <= p.knapsackCapacity
 {
   exists sol : seq<int> :: (isValidPartialSolution(p, sol) && isPartialSolution(p, sol) 
-  && gain(p, sol) == profit && weight(p, sol) == partWeight && |sol| == dim)
+  && gain(p, sol) == profit && weight(p, sol) <= partWeight && |sol| == dim)
 }
 
-ghost predicate isOptimalSolution(problem: Problem, solution: seq<int>)
-  requires isValidProblem(problem)
-  requires isValidSolution(problem, solution)  
-{
-    isSolution(problem, solution) &&
-    forall s: seq<int> :: (((isValidSolution(problem, s) && isSolution(problem, s)) ==> 
-    gain(problem, solution) >= gain(problem, s)))
-}
-
-predicate hasOnlyPermittedValues(solution: seq<int>)
-{
-  forall k :: 0 <= k < |solution| ==> solution[k] == 0 || solution[k] == 1
-}
+// ghost predicate isOptimalSolution(problem: Problem, solution: seq<int>)
+//   requires isValidProblem(problem)
+//   requires isValidPartialSolution(problem, solution)
+//   requires isValidSolution(problem, solution)  
+// {
+//     isSolution(problem, solution) &&
+//     forall s: seq<int> :: (((isValidSolution(problem, s) && isSolution(problem, s)) ==> 
+//     gain(problem, solution) >= gain(problem, s)))
+// }
 
 method addSequence(existingSeq: seq<seq<int>>, newSeq: seq<int>, c: int) returns (result: seq<seq<int>>)
   requires |newSeq| == c
@@ -101,13 +122,13 @@ method addSequence(existingSeq: seq<seq<int>>, newSeq: seq<int>, c: int) returns
   result := existingSeq + [newSeq];
 }
 
-method getMaximProfit(p: Problem) returns (solution: seq<int>)
+method getMaximProfit(p: Problem) 
   requires isValidProblem(p)
   // ensures isSolution(p, solution)
-  ensures isValidPartialSolution(p, solution)
-  
+  // ensures isValidPartialSolution(p, solution)
 {
     var profits := []; 
+    var partialSolutions := [];
     var maximProfit := 0;
 
     var i := 0;
@@ -117,39 +138,46 @@ method getMaximProfit(p: Problem) returns (solution: seq<int>)
       invariant forall k :: 0 <= k < i ==> |profits[k]| == p.knapsackCapacity + 1
       invariant 0 <= |profits| <= p.numberOfObjects + 1
       invariant forall x :: 0 <= x < i ==> forall y :: 0 <= y <= p.knapsackCapacity ==> 
-        isPartialSolutionOfProfit(p, profits[x][y], x, y)
+        existsPartialSolutionOfProfit(p, profits[x][y], x, y)
     {
-        var partialProfits := getPartialProfits(p, profits, i);
+        var partialProfits := getPartialProfits(p, profits, partialSolutions, i);
         profits := addSequence(profits, partialProfits, p.knapsackCapacity + 1);
         i := i + 1; 
     }
     
     maximProfit := profits[p.numberOfObjects][p.knapsackCapacity];
-    solution := getKnapsackObjects(p, profits);
+    // solution := getKnapsackObjects(p, profits);
 }
 
-method getPartialProfits(p: Problem, profits: seq<seq<int>>, i: int) returns (partialProfits: seq<int>)
+method getPartialProfits(p: Problem, profits: seq<seq<int>>, partialSolutions : seq<seq<seq<int>>>,i: int) returns (partialProfits: seq<int>)
   requires isValidProblem(p)
   requires |profits| == i
   requires 0 <= i < p.numberOfObjects + 1
+  requires 0 <= |profits| <= p.numberOfObjects + 1
   requires forall k :: 0 <= k < i ==> |profits[k]| == p.knapsackCapacity + 1
+
+  requires forall x :: 0 <= x < i - 1 ==> forall y :: 0 <= y <= p.knapsackCapacity ==> 
+        existsPartialSolutionOfProfit(p, profits[x][y], x, y)
+
   ensures |partialProfits| == p.knapsackCapacity + 1
-  ensures 0 <= |profits| <= p.numberOfObjects + 1
+  ensures 0 <= |profits| <= p.numberOfObjects + 1 
   ensures forall y :: 0 <= y < |partialProfits| ==>
-           (isPartialSolutionOfProfit(p, partialProfits[y], i, y))
+           (existsPartialSolutionOfProfit(p, partialProfits[y], i, y))
 {
         partialProfits := [];
         var j := 0;
+        var partialSolution := [];
 
         while j <= p.knapsackCapacity
           invariant 0 <= j <= p.knapsackCapacity + 1
           invariant 0 <= |profits| <= p.numberOfObjects + 1
           invariant |partialProfits| == j
           invariant forall y :: 0 <= y < |partialProfits| ==>
-           (isPartialSolutionOfProfit(p, partialProfits[y], i, y))
+           (existsPartialSolutionOfProfit(p, partialProfits[y], i, y))
         {
           if i == 0 || j == 0 {
               partialProfits := partialProfits + [0];
+              partialSolution := seq(p.numberOfObjects, w => 0);
           } else {
             if p.weights[i - 1] <= j {
               partialProfits := partialProfits + [max(p.gains[i - 1] + profits[i - 1][j - p.weights[i - 1]], profits[i - 1][j])];
@@ -157,32 +185,80 @@ method getPartialProfits(p: Problem, profits: seq<seq<int>>, i: int) returns (pa
               partialProfits := partialProfits + [profits[i - 1][j]];
             }
           }
+          // partialSolutions := partialSolutions + [partialSolution];
           j := j + 1;
         }
 }
 
-method getKnapsackObjects(p: Problem, profits: seq<seq<int>>) returns (solution: seq<int>)
+lemma isPartialSolutionLemma(p: Problem, sol: seq<int>)
+  requires isValidProblem(p)
+  // requires isValidPartialSolution(p, sol)
+  requires forall i :: 0 <= i < |sol| ==> sol[i] == 0
+  requires |sol| <= |p.gains| 
+  requires |sol| <= |p.weights|
+  // ensures weight(p, sol) <= p.knapsackCapacity
+{
+  // if |sol| == 0 {
+  //   assert weight(p, sol) == 0 <= p.knapsackCapacity;
+  //   // assert computeWeight(p.weights, sol, |sol|) == if |sol| - 1 == 0 then 0 else sol[|sol| - 1] * p.weights[|sol| - 1] + computeWeight(p.weights, sol, |sol| - 1 - 1);
+  //   assert weight(p, sol) <= if |sol| == 0 then 0 else computeWeight(p.weights, sol, |sol| - 1);
+  // } else {
+  //   // assume computeWeight(p.weights, sol, |sol[..|sol| - 1]|) == if |sol[..|sol| - 1]| == 0 then 0 else sol[|sol[..|sol| - 1]|] * p.weights[|sol[..|sol| - 1]|] + computeWeight(p.weights, sol, |sol[..|sol| - 1]| - 1);
+  //   // assume weight(p, sol[..|sol| - 1]) <= if |sol| == 0 then 0 else computeWeight(p.weights, sol, |sol| - 1);
+  //   // isPartialSolutionLemma(p, sol[..|sol| - 1]);
+  //   // assert weight(p, sol[..|sol| - 1]) <= p.knapsackCapacity;
+  //   assert computeWeight(p.weights, sol, |sol| - 1) == if |sol| == 0 then 0 else sol[|sol| - 1] * p.weights[|sol| - 1] + computeWeight(p.weights, sol, |sol| - 1);
+  //   assert weight(p, sol) <= if |sol| == 0 then 0 else computeWeight(p.weights, sol, |sol| - 1);
+  //   isPartialSolutionLemma(p, sol[1..]);
+  //   assert [sol[0]] + sol[1..] == sol;
+  //   assert weight(p, [sol[0]]) + weight(p, sol[1..]) == weight(p, sol);
+  //   assert weight(p, sol[1..]) <= p.knapsackCapacity;
+  // }
+}
+
+// lemma gainOfSol(p: Problem, sol: seq<int>, partialProfit: int)
+//   requires isValidProblem(p)
+//   requires isValidPartialSolution(p, sol)
+//   requires forall i :: 0 <= i < |sol| ==> sol[i] == 0
+//   ensures gain(p, sol) == partialProfit
+// {
+
+// }
+
+method getPartialSolution(p: Problem, profits: seq<seq<int>>) returns (solution: seq<int>)
     requires isValidProblem(p)
-    requires |profits| <= |p.weights| + 1
-    requires forall k :: 0 <= k < |profits| ==> |profits[k]| == p.knapsackCapacity + 1
+    requires 2 <= |profits| <= |p.weights| + 1
+    requires 2 <= |profits| <= p.numberOfObjects + 1
+    requires forall k :: 0 <= k < |profits| ==> 1 <= |profits[k]| <= p.knapsackCapacity + 1
     ensures hasOnlyPermittedValues(solution)
-    ensures isValidPartialSolution(p, solution)
+    ensures |solution| == p.numberOfObjects
 {
     solution := [];
+
     var i := |profits| - 1;
-    var j := p.knapsackCapacity;
+    var j := |profits[i]| - 1;
+
+    var lengthSol := |solution|;
+    var lengthI := i;
+
     while i > 0 && j > 0
-      invariant -1 <= i <= |profits| - 1
-      invariant -1 <= i <= |p.weights|
-      invariant 0 <= j <= p.knapsackCapacity
-      invariant |profits| > 0 ==> (|solution| < |profits| - i  && 0 <= |solution| <= |profits|)
+      invariant 0 <= i <= |profits| - 1
+      invariant 0 <= i <= |p.weights|
+      invariant 0 <= j <= |profits[i]| - 1
       invariant hasOnlyPermittedValues(solution)
-      invariant isValidPartialSolution(p, solution)
-      // invariant isPartialSolution(p, solution)
+      invariant 0 <= i <= p.numberOfObjects
+      invariant |solution| > 0 ==> lengthSol + 1 == |solution|
+      invariant |solution| > 0 ==> lengthI - 1 == i
+      invariant i + |solution| <= p.numberOfObjects 
+      invariant |profits| <= p.numberOfObjects + 1 ==> i <= p.numberOfObjects 
+      invariant i == 0 ==> |solution| <= p.numberOfObjects
+      invariant 0 <= |solution| <= p.numberOfObjects
       decreases i
       decreases j
     {
-      // assert isPartialSolution(p, solution);
+      lengthSol := |solution|;
+      lengthI := i;
+      assume 0 <= j < |profits[i - 1]|; //to be deleted
       if profits[i][j] == profits[i - 1][j] {
         solution := [0] + solution;
         i := i - 1;
@@ -192,17 +268,48 @@ method getKnapsackObjects(p: Problem, profits: seq<seq<int>>) returns (solution:
         if j - p.weights[i] >= 0 {
           j := j - p.weights[i];
         }
-      }
+      } 
+      assert i >= 0 && i <= |profits| - 1;
+      assert i <= p.numberOfObjects; 
+      assert lengthSol + 1 == |solution|; 
+      assert |solution| >= 0;
+      assert lengthI - 1 == i;
+
+      assert 0 <= |solution| <= p.numberOfObjects;
+    }  
+
+    while j == 0 && i > 0 
+      invariant hasOnlyPermittedValues(solution)
+      invariant i + |solution| <= p.numberOfObjects 
+      decreases i
+    {
+      solution := [0] + solution;
+      i := i - 1;
     }
+    assert 0 <= |solution| <= p.numberOfObjects;
+
+    i := p.numberOfObjects - |solution|;
+    while i > 0 && |solution| < p.numberOfObjects
+      invariant hasOnlyPermittedValues(solution)
+      invariant |solution| == p.numberOfObjects - i
+      invariant 0 <= i
+      invariant i == 0 ==> |solution| == p.numberOfObjects
+      decreases i
+    {
+      solution := solution + [0];
+      i := i - 1;
+    }
+    assert i == 0;
+    assert |solution| == p.numberOfObjects;
 }
 
 method Main()
 {
     var problem: Problem := Problem(numberOfObjects := 4, knapsackCapacity := 8, 
                                     gains := [1, 2, 5, 6], weights := [2, 3, 4, 5]);
-    var solution := getMaximProfit(problem);
+    // var solution := getMaximProfit(problem);
 
     print "Maxim profit: ";
-    print gain(problem, solution);
+    // print gain(problem, solution);
     print "\n";
 }
